unity/models/nondet.lean
@@ -1,0 +1,223 @@
+
+import unity.logic
+import unity.temporal
+
+import util.logic
+
+universe variable u
+namespace nondet
+
+section nondet
+
+open predicate
+
+parameter {α : Type}
+
+def pred := α → Prop
+
+structure event : Type :=
+  (coarse_sch : pred)
+  (fine_sch : pred)
+  (step : ∀ s, coarse_sch s → fine_sch s → α → Prop)
+  (fis : ∀ s CS FS, ∃ s', step s CS FS s')
+
+structure prog (lbl : Type) : Type :=
+  (first : α → Prop)
+  (first_fis : ∃ s, first s)
+  (event' : lbl → event)
+
+variables {lbl : Type}
+
+def skip : event :=
+{ coarse_sch := True
+, fine_sch := True
+, step := λ s _ _ s', s = s'
+, fis := take s _ _, ⟨s,rfl⟩ }
+
+def prog.event (s : prog lbl) : option lbl → event
+  | none := skip
+  | (some e) := s^.event' e
+
+def prog.init (s : prog lbl) (p : pred) : Prop
+:= s^.first ⟹ p
+
+def prog.guard  (s : prog lbl) (e : option lbl) : α → Prop :=
+(s^.event e)^.coarse_sch && (s^.event e)^.fine_sch
+
+def prog.take_step (s : prog lbl) : ∀ (e : option lbl) (σ : α), s^.guard e σ → α → Prop
+  | none σ _ := λ σ', σ = σ'
+  | (some e) σ p := (s^.event e)^.step σ p.left p.right
+
+open temporal
+
+def prog.coarse_sch_of (s : prog lbl) (act : option lbl) : α → Prop :=
+(s.event act).coarse_sch
+
+def prog.fine_sch_of (s : prog lbl) (act : option lbl) : α → Prop :=
+(s.event act).fine_sch
+
+def prog.step_of (s : prog lbl) (act : option lbl) : α → α → Prop :=
+λ σ σ', ∃ guard, s.take_step act σ guard σ'
+
+def is_step (s : prog lbl) (σ σ' : α) : Prop :=
+∃ ev, s.step_of ev σ σ'
+
+structure prog.ex (s : prog lbl) (τ : stream α) : Prop :=
+    (init : s^.first (τ 0))
+    (safety : ∀ i, ⟦ is_step s ⟧ (τ.drop i))
+    (liveness : ∀ e, (<>[]• s^.coarse_sch_of e) τ →
+                     ([]<>• s^.fine_sch_of e) τ →
+                     ([]<> ⟦ s.step_of e ⟧) τ)
+
+structure prog.falsify (s : prog lbl) (act : option lbl) (p : pred' α) : Prop :=
+  (enable : p ⟹ s^.coarse_sch_of act)
+  (schedule : prog.ex s ⟹ (<>[]•p ⟶ []<>• s^.fine_sch_of act) )
+  (negate' : ⦃ •p ⟶ ⟦ s^.step_of act ⟧ ⟶ ⟦ λ _, ~p ⟧ ⦄)
+
+open temporal
+
+lemma prog.falsify.negate
+   {s : prog lbl} {act : option lbl} {p : pred' α}
+:  prog.falsify s act p
+→  •p && ⟦ s^.step_of act ⟧ ⟹ <>~•p :=
+begin
+  intros h₀ τ h₁,
+  note h₂ := h₀.negate' _ h₁^.left h₁^.right,
+  unfold eventually p_not init,
+  existsi 1,
+  apply h₂,
+end
+
+def prog.transient (s : prog lbl) (p : pred' α) : Prop :=
+∃ (act : option lbl), prog.falsify s act p
+
+section theorems
+
+variable (s : prog lbl)
+
+open prog
+open event
+
+theorem prog.transient_false : transient s False :=
+begin
+  unfold prog.transient,
+  existsi none,
+  apply falsify.mk,
+  { intros σ h, cases h },
+  { intros τ i h₀ h₁,
+    simp at h₀,
+    cases h₀, },
+  { intros σ h₀ h₁, cases h₀ with h₂ }
+end
+
+def prog.transient_str : ∀ (s : prog lbl) {p q : α → Prop}, (∀ (i : α), p i → q i) → prog.transient s q → prog.transient s p :=
+begin
+  intros s p q h,
+  unfold transient,
+  apply exists_imp_exists,
+  intros e h',
+  apply falsify.mk,
+  { apply forall_imp_forall _ h'.enable,
+    intro x,
+    apply imp_imp_imp_left,
+    apply h },
+  { apply forall_imp_forall _ h'.schedule,
+    intro τ,
+    apply forall_imp_forall _,
+    intro j,
+    apply p_imp_p_imp_p_imp_left _,
+    apply ex_map,
+    apply hence_map,
+    apply init_map,
+    apply h },
+  { apply forall_imp_forall _ h'.negate',
+    intro τ,
+    apply imp_mono _ _,
+    { apply h },
+    apply imp_imp_imp_right _,
+    apply next_imp_next _ _,
+    apply entail_contrapos,
+    apply h }
+end
+
+end theorems
+
+instance prog_is_system : unity.system (prog lbl) :=
+{ σ := α
+, transient := @prog.transient lbl
+, step := is_step
+, init   := prog.init
+, transient_false := prog.transient_false
+, transient_str := prog.transient_str }
+
+section soundness
+
+open prog
+
+variables {s : prog lbl} {p : pred' α}
+variables (T₀ : prog.transient s p)
+include T₀
+variables (τ : stream α)
+
+lemma transient.semantics (h : ex s τ)
+: ([]<>~•p) τ :=
+begin
+  cases (temporal.em' (•p) τ) with h_p ev_np,
+  { unfold prog.transient at T₀,
+    cases T₀ with ev T₀,
+    assert Hc : (<>[]•s.coarse_sch_of ev) τ,
+    { apply ex_map _ _ h_p,
+      apply hence_map _ ,
+      apply init_map _ ,
+      apply T₀.enable },
+    assert Hf : ([]<>•s.fine_sch_of ev) τ,
+    { apply T₀.schedule _ h h_p, },
+    note act := coincidence h_p (h.liveness ev Hc Hf),
+    rw [-eventually_eventually],
+    apply hence_map _ _ act,
+    apply ex_map _ ,
+    apply T₀.negate },
+  { apply ev_np },
+end
+
+end soundness
+
+-- instance {α} [sched lbl] : system_sem (prog lbl) :=
+instance : unity.system_sem (prog lbl) :=
+  { (_ : unity.system (prog lbl)) with
+    ex := prog.ex
+  , safety := @prog.ex.safety _ _
+  , inhabited := sorry
+  , transient_sem := @transient.semantics _ }
+
+open unity
+
+theorem transient_rule {s : prog lbl} {p : pred' α} (ev : option lbl)
+   (EN : p ⟹ s.coarse_sch_of ev)
+   (FLW : leads_to s (p && s.coarse_sch_of ev) (s.fine_sch_of ev))
+   (NEG : ∀ σ σ', p σ → s.step_of ev σ σ' → ¬p σ')
+: s.transient p :=
+begin
+  unfold prog.transient,
+  existsi ev,
+  apply falsify.mk,
+    -- enablement
+  { apply EN },
+    -- follow
+  { intros τ sem H,
+    apply inf_often_of_leads_to (system_sem.leads_to_sem FLW _ sem),
+    note H' := inf_often_of_stable _ H,
+    apply hence_map _ _ H',
+    apply ex_map _ ,
+    apply init_map _ ,
+    intros σ Hp,
+    apply and.intro Hp,
+    apply EN _ Hp },
+    -- negation
+  { intros σ Hp Hact,
+    apply NEG _ _ Hp Hact }
+end
+
+end nondet
+
+end nondet
